Update extracted files for libcrux-ml-kem

libcrux-ml-kem/proofs/fstar/extraction/Libcrux_ml_kem.Hash_functions.Avx2.fsti
@@ -9,7 +9,7 @@ open FStar.Mul
 type t_Simd256Hash = { f_shake128_state:Libcrux_sha3.Avx2.X4.Incremental.t_KeccakState4 }
 
 [@@ FStar.Tactics.Typeclasses.tcinstance]
-let impl (v_K: usize) : Libcrux_ml_kem.Hash_functions.t_Hash t_Simd256Hash v_K =
+let impl (v_K: usize) : Libcrux_ml_kem.Hash_functions.t_Hash #t_Simd256Hash v_K =
   {
     f_G_pre = (fun (input: t_Slice u8) -> true);
     f_G_post = (fun (input: t_Slice u8) (out: t_Array u8 (sz 64)) -> true);
