libcrux-ml-kem/proofs/fstar/extraction/Libcrux_ml_kem.Ind_cca.Instantiations.Portable.fsti
@@ -7,7 +7,7 @@ let _ =
   (* This module has implicit dependencies, here we make them explicit. *)
   (* The implicit dependencies arise from typeclasses instances. *)
   let open Libcrux_ml_kem.Hash_functions.Portable in
-  let open Libcrux_ml_kem.Vector in
+  let open Libcrux_ml_kem.Vector.Portable in
   ()
 
 /// Portable decapsulate
