libcrux-ml-kem/proofs/fstar/extraction/Libcrux_ml_kem.Vector.Portable.Vector_type.fsti
@@ -1,0 +1,16 @@
+module Libcrux_ml_kem.Vector.Portable.Vector_type
+#set-options "--fuel 0 --ifuel 1 --z3rlimit 15"
+open Core
+open FStar.Mul
+
+/// Values having this type hold a representative 'x' of the Kyber field.
+/// We use 'fe' as a shorthand for this type.
+unfold
+let t_FieldElement = i16
+
+type t_PortableVector = { f_elements:t_Array i16 (sz 16) }
+
+val from_i16_array (array: t_Slice i16)
+    : Prims.Pure t_PortableVector Prims.l_True (fun _ -> Prims.l_True)
+
+val zero: Prims.unit -> Prims.Pure t_PortableVector Prims.l_True (fun _ -> Prims.l_True)
