libcrux-ml-kem/proofs/fstar/extraction/Libcrux_ml_kem.Vector.Traits.fsti
@@ -3,7 +3,7 @@ module Libcrux_ml_kem.Vector.Traits
 open Core
 open FStar.Mul
 
-class t_Operations (v_Self: Type0) = {
+class t_Operations (#v_Self: Type0) = {
   [@@@ FStar.Tactics.Typeclasses.no_method]_super_11581440318597584651:Core.Marker.t_Copy v_Self;
   [@@@ FStar.Tactics.Typeclasses.no_method]_super_9442900250278684536:Core.Clone.t_Clone v_Self;
   f_ZERO_pre:Prims.unit -> bool;
